format-version: 1.2
data-version: phases/releases/2025-05-10/phases-base.owl
idspace: dc http://purl.org/dc/elements/1.1/ 
idspace: terms http://purl.org/dc/terms/ 
ontology: phases/phases-base
property_value: dc:type IAO:8000001
property_value: owl:versionInfo "2025-05-10" xsd:string
property_value: terms:contributor https://orcid.org/0000-0001-6906-5548
property_value: terms:contributor https://orcid.org/0000-0001-9189-9661
property_value: terms:contributor https://orcid.org/0000-0001-9625-1899
property_value: terms:contributor https://orcid.org/0000-0002-1118-1738
property_value: terms:contributor https://orcid.org/0000-0002-2999-0103
property_value: terms:contributor https://orcid.org/0000-0003-2294-3571
property_value: terms:contributor https://orcid.org/0009-0009-9778-4641
property_value: terms:description "PHASES provides an ontology for integrating research in solitude and gerotranscendence. By integrating these areas of study, we aim to deepen our understanding of each and how they promote healthy aging." xsd:string
property_value: terms:license https://creativecommons.org/publicdomain/zero/1.0/
property_value: terms:title "Promoting Health Aging through Semantic Enrichment of Solitude Research (PHASES) Ontology" xsd:string

[Term]
id: PHASES:0000000
name: reminiscence therapy
def: "A behavior change intervention that uses life histories—written, oral, or both—to improve psychological well-being. The therapy is often used with older people." [] {IAO:0000119="https://dictionary.apa.org/reminiscence-therapy"}
is_a: BCIO:003000
property_value: terms:contributor https://orcid.org/0000-0001-6906-5548
property_value: terms:contributor https://orcid.org/0000-0001-9625-1899
property_value: terms:created "2025-03-03T21:39:49Z" xsd:dateTime

[Term]
id: PHASES:0002000
name: solitude
def: "A mental disposition that, if realized, is realized in being physical alone or in lacking social interactions, whether desired or not." [] {IAO:0000119="Oliveira, J., Guerra, S., Sousa, L., & Ribeiro, O. (2024). Solitude in old age: a scoping review of conceptualisations, associated factors and impacts. Aging & Mental Health, 29(2), 220–227. https://doi.org/10.1080/13607863.2024.2379408"}
is_a: MF:0000033
property_value: terms:contributor https://orcid.org/0000-0001-6906-5548
property_value: terms:created "2025-02-05T17:49:47Z" xsd:dateTime

[Term]
id: PHASES:0002001
name: gerotranscendence
def: "A mental disposition borne by older adults such that, if realized, is realized in shifting in goals, values, and perspectives towards connections to past and future generations and in seeking coherence in one's life narrative." [] {IAO:0000119="https://pmc.ncbi.nlm.nih.gov/articles/PMC10466938/"}
is_a: MF:0000033
property_value: terms:contributor https://orcid.org/0000-0001-6906-5548
property_value: terms:created "2025-02-05T17:54:30Z" xsd:dateTime

[Term]
id: PHASES:0002002
name: social isolation
def: "Social alienation that, if realized, is realized in being physically alone and desiring not to be." [] {IAO:0000119="https://www.nia.nih.gov/health/loneliness-and-social-isolation/loneliness-and-social-isolation-tips-staying-connected"}
is_a: BCIO:006014
property_value: terms:contributor https://orcid.org/0000-0001-6906-5548
property_value: terms:created "2025-02-26T21:16:23Z" xsd:dateTime

[Term]
id: PHASES:0002003
name: loneliness
def: "A subjective affective feeling of dissatisfaction with a lack of social interactions and relationships." [] {IAO:0000119="Asher, S. R., Hymel, S., & Renshaw, P. D. (1984). Loneliness in children. Child development, 1456-1464."}
is_a: MFOEM:000006
property_value: terms:contributor https://orcid.org/0000-0001-6906-5548
property_value: terms:created "2025-02-05T17:58:33Z" xsd:dateTime

[Term]
id: PHASES:0002004
name: theory
def: "An information content entity that is a principle or body of interrelated principles that purports to explain or predict a number of interrelated phenomena." [] {IAO:0000119="https://dictionary.apa.org/theory"}
is_a: IAO:0000030
property_value: terms:contributor https://orcid.org/0000-0001-6906-5548
property_value: terms:created "2025-02-26T21:20:31Z" xsd:dateTime

[Term]
id: PHASES:0002005
name: psychological theory
def: "A theory that summarizes and explains mental and behavioral patterns within the context of society and culture." [] {IAO:0000119="https://www.sciencedirect.com/topics/psychology/psychological-theory"}
is_a: PHASES:0002004 ! theory
property_value: terms:contributor https://orcid.org/0000-0001-6906-5548
property_value: terms:created "2025-02-26T21:20:56Z" xsd:dateTime

[Term]
id: PHASES:0002006
name: social convoy model
def: "A psychological theory positing that social connections differ in levels of closeness and stability, where peripheral relationships are most vulnerable to change and termination, especially with increased age." [] {IAO:0000119="Antonucci, T. C., Ajrouch, K. J., & Birditt, K. S. (2014). The convoy model: Explaining social relations from a multidisciplinary perspective. The Gerontologist, 54(1), 82-92."}
is_a: PHASES:0002005 ! psychological theory
property_value: terms:contributor https://orcid.org/0000-0001-6906-5548
property_value: terms:created "2025-02-26T21:21:13Z" xsd:dateTime

[Term]
id: PHASES:0002007
name: ego integrity
def: "A psychological theory that posits the acceptance of life as it has been lived, including acceptance of death, as the major driving psychological goal of older adults." [] {IAO:0000119="Erikson E.H. The Life Cycle Completed. Norton; New York, NY, USA: 1982."}
is_a: PHASES:0002005 ! psychological theory
property_value: terms:contributor https://orcid.org/0000-0001-6906-5548
property_value: terms:created "2025-02-26T21:24:11Z" xsd:dateTime

[Term]
id: PHASES:0002008
name: self-transcendence theory
def: "A psychological theory that posits self-transcendence as a mediating role between vulnerability and well-being, influenced by personal and contextual factors." [] {IAO:0000119="Reed, P.G. (1991). Toward a nursing theory of self-transcendence: Deductive reformulation using developmental theories. Advances in Nursing Science, 13 (4), 64-77."}
is_a: PHASES:0002005 ! psychological theory
property_value: terms:contributor https://orcid.org/0000-0001-6906-5548
property_value: terms:created "2025-02-26T21:26:30Z" xsd:dateTime

