<?xml version="1.0"?>
<rdf:RDF xmlns="http://purl.obolibrary.org/obo/phases/imports/ro_import.owl#"
     xml:base="http://purl.obolibrary.org/obo/phases/imports/ro_import.owl"
     xmlns:dc="http://purl.org/dc/elements/1.1/"
     xmlns:obo="http://purl.obolibrary.org/obo/"
     xmlns:owl="http://www.w3.org/2002/07/owl#"
     xmlns:rdf="http://www.w3.org/1999/02/22-rdf-syntax-ns#"
     xmlns:xml="http://www.w3.org/XML/1998/namespace"
     xmlns:xsd="http://www.w3.org/2001/XMLSchema#"
     xmlns:rdfs="http://www.w3.org/2000/01/rdf-schema#">
    <owl:Ontology rdf:about="http://purl.obolibrary.org/obo/phases/imports/ro_import.owl">
        <owl:versionIRI rdf:resource="http://purl.obolibrary.org/obo/phases/imports/ro_import.owl"/>
    </owl:Ontology>
    


    <!-- 
    ///////////////////////////////////////////////////////////////////////////////////////
    //
    // Annotation properties
    //
    ///////////////////////////////////////////////////////////////////////////////////////
     -->

    


    <!-- http://purl.obolibrary.org/obo/IAO_0000111 -->

    <owl:AnnotationProperty rdf:about="http://purl.obolibrary.org/obo/IAO_0000111">
        <obo:IAO_0000111 xml:lang="en">editor preferred term</obo:IAO_0000111>
        <obo:IAO_0000114 rdf:resource="http://purl.obolibrary.org/obo/IAO_0000122"/>
        <obo:IAO_0000115 xml:lang="en">The concise, meaningful, and human-friendly name for a class or property preferred by the ontology developers. (US-English)</obo:IAO_0000115>
        <obo:IAO_0000117 xml:lang="en">PERSON:Daniel Schober</obo:IAO_0000117>
        <obo:IAO_0000119 xml:lang="en">GROUP:OBI:&lt;http://purl.obolibrary.org/obo/obi&gt;</obo:IAO_0000119>
        <rdfs:isDefinedBy rdf:resource="http://purl.obolibrary.org/obo/phases/imports/ro_import.owl"/>
        <rdfs:label xml:lang="en">editor preferred term</rdfs:label>
    </owl:AnnotationProperty>
    


    <!-- http://purl.obolibrary.org/obo/IAO_0000112 -->

    <owl:AnnotationProperty rdf:about="http://purl.obolibrary.org/obo/IAO_0000112">
        <obo:IAO_0000111 xml:lang="en">example of usage</obo:IAO_0000111>
        <obo:IAO_0000114 rdf:resource="http://purl.obolibrary.org/obo/IAO_0000122"/>
        <obo:IAO_0000115 xml:lang="en">A phrase describing how a term should be used and/or a citation to a work which uses it. May also include other kinds of examples that facilitate immediate understanding, such as widely know prototypes or instances of a class, or cases where a relation is said to hold.</obo:IAO_0000115>
        <obo:IAO_0000117 xml:lang="en">PERSON:Daniel Schober</obo:IAO_0000117>
        <obo:IAO_0000119 xml:lang="en">GROUP:OBI:&lt;http://purl.obolibrary.org/obo/obi&gt;</obo:IAO_0000119>
        <rdfs:isDefinedBy rdf:resource="http://purl.obolibrary.org/obo/phases/imports/ro_import.owl"/>
        <rdfs:label>example of usage</rdfs:label>
        <rdfs:label xml:lang="en">example of usage</rdfs:label>
    </owl:AnnotationProperty>
    


    <!-- http://purl.obolibrary.org/obo/IAO_0000114 -->

    <owl:AnnotationProperty rdf:about="http://purl.obolibrary.org/obo/IAO_0000114">
        <obo:IAO_0000111 xml:lang="en">has curation status</obo:IAO_0000111>
        <obo:IAO_0000117 xml:lang="en">PERSON:Alan Ruttenberg</obo:IAO_0000117>
        <obo:IAO_0000117 xml:lang="en">PERSON:Bill Bug</obo:IAO_0000117>
        <obo:IAO_0000117 xml:lang="en">PERSON:Melanie Courtot</obo:IAO_0000117>
        <rdfs:isDefinedBy rdf:resource="http://purl.obolibrary.org/obo/phases/imports/ro_import.owl"/>
        <rdfs:label xml:lang="en">has curation status</rdfs:label>
    </owl:AnnotationProperty>
    


    <!-- http://purl.obolibrary.org/obo/IAO_0000115 -->

    <owl:AnnotationProperty rdf:about="http://purl.obolibrary.org/obo/IAO_0000115">
        <obo:IAO_0000111 xml:lang="en">definition</obo:IAO_0000111>
        <obo:IAO_0000114 rdf:resource="http://purl.obolibrary.org/obo/IAO_0000122"/>
        <obo:IAO_0000115 xml:lang="en">The official definition, explaining the meaning of a class or property. Shall be Aristotelian, formalized and normalized. Can be augmented with colloquial definitions.</obo:IAO_0000115>
        <obo:IAO_0000116 xml:lang="en">2012-04-05: 
Barry Smith

The official OBI definition, explaining the meaning of a class or property: &apos;Shall be Aristotelian, formalized and normalized. Can be augmented with colloquial definitions&apos;  is terrible.

Can you fix to something like:

A statement of necessary and sufficient conditions explaining the meaning of an expression referring to a class or property.

Alan Ruttenberg

Your proposed definition is a reasonable candidate, except that it is very common that necessary and sufficient conditions are not given. Mostly they are necessary, occasionally they are necessary and sufficient or just sufficient. Often they use terms that are not themselves defined and so they effectively can&apos;t be evaluated by those criteria. 

On the specifics of the proposed definition:

We don&apos;t have definitions of &apos;meaning&apos; or &apos;expression&apos; or &apos;property&apos;. For &apos;reference&apos; in the intended sense I think we use the term &apos;denotation&apos;. For &apos;expression&apos;, I think we you mean symbol, or identifier. For &apos;meaning&apos; it differs for class and property. For class we want documentation that let&apos;s the intended reader determine whether an entity is instance of the class, or not. For property we want documentation that let&apos;s the intended reader determine, given a pair of potential relata, whether the assertion that the relation holds is true. The &apos;intended reader&apos; part suggests that we also specify who, we expect, would be able to understand the definition, and also generalizes over human and computer reader to include textual and logical definition. 

Personally, I am more comfortable weakening definition to documentation, with instructions as to what is desirable. 

We also have the outstanding issue of how to aim different definitions to different audiences. A clinical audience reading chebi wants a different sort of definition documentation/definition from a chemistry trained audience, and similarly there is a need for a definition that is adequate for an ontologist to work with.  </obo:IAO_0000116>
        <obo:IAO_0000117 xml:lang="en">PERSON:Daniel Schober</obo:IAO_0000117>
        <obo:IAO_0000119 xml:lang="en">GROUP:OBI:&lt;http://purl.obolibrary.org/obo/obi&gt;</obo:IAO_0000119>
        <rdfs:isDefinedBy rdf:resource="http://purl.obolibrary.org/obo/phases/imports/ro_import.owl"/>
        <rdfs:label>definition</rdfs:label>
        <rdfs:label xml:lang="en">definition</rdfs:label>
    </owl:AnnotationProperty>
    


    <!-- http://purl.obolibrary.org/obo/IAO_0000116 -->

    <owl:AnnotationProperty rdf:about="http://purl.obolibrary.org/obo/IAO_0000116">
        <obo:IAO_0000111 xml:lang="en">editor note</obo:IAO_0000111>
        <obo:IAO_0000114 rdf:resource="http://purl.obolibrary.org/obo/IAO_0000122"/>
        <obo:IAO_0000115 xml:lang="en">An administrative note intended for its editor. It may not be included in the publication version of the ontology, so it should contain nothing necessary for end users to understand the ontology.</obo:IAO_0000115>
        <obo:IAO_0000117 xml:lang="en">PERSON:Daniel Schober</obo:IAO_0000117>
        <obo:IAO_0000119 xml:lang="en">GROUP:OBI:&lt;http://purl.obofoundry.org/obo/obi&gt;</obo:IAO_0000119>
        <rdfs:isDefinedBy rdf:resource="http://purl.obolibrary.org/obo/phases/imports/ro_import.owl"/>
        <rdfs:label xml:lang="en">editor note</rdfs:label>
    </owl:AnnotationProperty>
    


    <!-- http://purl.obolibrary.org/obo/IAO_0000117 -->

    <owl:AnnotationProperty rdf:about="http://purl.obolibrary.org/obo/IAO_0000117">
        <obo:IAO_0000111 xml:lang="en">term editor</obo:IAO_0000111>
        <obo:IAO_0000114 rdf:resource="http://purl.obolibrary.org/obo/IAO_0000122"/>
        <obo:IAO_0000115 xml:lang="en">Name of editor entering the term in the file. The term editor is a point of contact for information regarding the term. The term editor may be, but is not always, the author of the definition, which may have been worked upon by several people</obo:IAO_0000115>
        <obo:IAO_0000116 xml:lang="en">20110707, MC: label update to term editor and definition modified accordingly. See https://github.com/information-artifact-ontology/IAO/issues/115.</obo:IAO_0000116>
        <obo:IAO_0000117 xml:lang="en">PERSON:Daniel Schober</obo:IAO_0000117>
        <obo:IAO_0000119 xml:lang="en">GROUP:OBI:&lt;http://purl.obolibrary.org/obo/obi&gt;</obo:IAO_0000119>
        <rdfs:isDefinedBy rdf:resource="http://purl.obolibrary.org/obo/phases/imports/ro_import.owl"/>
        <rdfs:label xml:lang="en">term editor</rdfs:label>
    </owl:AnnotationProperty>
    


    <!-- http://purl.obolibrary.org/obo/IAO_0000119 -->

    <owl:AnnotationProperty rdf:about="http://purl.obolibrary.org/obo/IAO_0000119">
        <obo:IAO_0000111 xml:lang="en">definition source</obo:IAO_0000111>
        <obo:IAO_0000114 rdf:resource="http://purl.obolibrary.org/obo/IAO_0000122"/>
        <obo:IAO_0000115 xml:lang="en">Formal citation, e.g. identifier in external database to indicate / attribute source(s) for the definition. Free text indicate / attribute source(s) for the definition. EXAMPLE: Author Name, URI, MeSH Term C04, PUBMED ID, Wiki uri on 31.01.2007</obo:IAO_0000115>
        <obo:IAO_0000117 xml:lang="en">PERSON:Daniel Schober</obo:IAO_0000117>
        <obo:IAO_0000119 xml:lang="en">Discussion on obo-discuss mailing-list, see http://bit.ly/hgm99w</obo:IAO_0000119>
        <obo:IAO_0000119 xml:lang="en">GROUP:OBI:&lt;http://purl.obolibrary.org/obo/obi&gt;</obo:IAO_0000119>
        <rdfs:isDefinedBy rdf:resource="http://purl.obolibrary.org/obo/phases/imports/ro_import.owl"/>
        <rdfs:label xml:lang="en">definition source</rdfs:label>
    </owl:AnnotationProperty>
    


    <!-- http://purl.obolibrary.org/obo/IAO_0000233 -->

    <owl:AnnotationProperty rdf:about="http://purl.obolibrary.org/obo/IAO_0000233">
        <obo:IAO_0000111 xml:lang="en">term tracker item</obo:IAO_0000111>
        <obo:IAO_0000112 xml:lang="en">the URI for an OBI Terms ticket at sourceforge, such as https://sourceforge.net/p/obi/obi-terms/772/</obo:IAO_0000112>
        <obo:IAO_0000114 rdf:resource="http://purl.obolibrary.org/obo/IAO_0000125"/>
        <obo:IAO_0000115 xml:lang="en">An IRI or similar locator for a request or discussion of an ontology term.</obo:IAO_0000115>
        <obo:IAO_0000117 xml:lang="en">Person: Jie Zheng, Chris Stoeckert, Alan Ruttenberg</obo:IAO_0000117>
        <obo:IAO_0000119 xml:lang="en">Person: Jie Zheng, Chris Stoeckert, Alan Ruttenberg</obo:IAO_0000119>
        <rdfs:comment xml:lang="en">The &apos;tracker item&apos; can associate a tracker with a specific ontology term.</rdfs:comment>
        <rdfs:isDefinedBy rdf:resource="http://purl.obolibrary.org/obo/phases/imports/ro_import.owl"/>
        <rdfs:label xml:lang="en">term tracker item</rdfs:label>
    </owl:AnnotationProperty>
    


    <!-- http://purl.obolibrary.org/obo/IAO_0000425 -->

    <owl:AnnotationProperty rdf:about="http://purl.obolibrary.org/obo/IAO_0000425">
        <obo:IAO_0000111 xml:lang="en">expand assertion to</obo:IAO_0000111>
        <obo:IAO_0000112 xml:lang="en">ObjectProperty: RO???
Label: spatially disjoint from
Annotations: expand_assertion_to &quot;DisjointClasses: (http://purl.obolibrary.org/obo/BFO_0000051 some ?X)  (http://purl.obolibrary.org/obo/BFO_0000051 some ?Y)&quot;
</obo:IAO_0000112>
        <obo:IAO_0000115 xml:lang="en">A macro expansion tag applied to an annotation property which can be expanded into a more detailed axiom.</obo:IAO_0000115>
        <obo:IAO_0000117 xml:lang="en">Chris Mungall</obo:IAO_0000117>
        <rdfs:isDefinedBy rdf:resource="http://purl.obolibrary.org/obo/phases/imports/ro_import.owl"/>
        <rdfs:label xml:lang="en">expand assertion to</rdfs:label>
    </owl:AnnotationProperty>
    


    <!-- http://purl.obolibrary.org/obo/OMO_0002000 -->

    <owl:AnnotationProperty rdf:about="http://purl.obolibrary.org/obo/OMO_0002000">
        <obo:IAO_0000112>&apos;part disjoint with&apos; &apos;defined by construct&apos; &quot;&quot;&quot;
    PREFIX owl: &lt;http://www.w3.org/2002/07/owl#&gt;
    PREFIX : &lt;http://example.org/
    CONSTRUCT {
      [
        a owl:Restriction ;
        owl:onProperty :part_of ;
        owl:someValuesFrom ?a ;
        owl:disjointWith [
          a owl:Restriction ;
          owl:onProperty :part_of ;
          owl:someValuesFrom ?b
        ]
      ]
    }
    WHERE {
      ?a :part_disjoint_with ?b .
    }</obo:IAO_0000112>
        <obo:IAO_0000115>Links an annotation property to a SPARQL CONSTRUCT query which is meant to provide semantics for a shortcut relation.</obo:IAO_0000115>
        <obo:IAO_0000233 rdf:resource="https://github.com/ontodev/robot/issues/963"/>
        <dc:contributor rdf:resource="https://orcid.org/0000-0002-7356-1779"/>
        <dc:contributor rdf:resource="https://orcid.org/0000-0002-8688-6599"/>
        <rdfs:isDefinedBy rdf:resource="http://purl.obolibrary.org/obo/phases/imports/ro_import.owl"/>
        <rdfs:label>defined by construct</rdfs:label>
    </owl:AnnotationProperty>
    


    <!-- http://purl.obolibrary.org/obo/RO_0002161 -->

    <owl:AnnotationProperty rdf:about="http://purl.obolibrary.org/obo/RO_0002161">
        <obo:IAO_0000112>tooth SubClassOf &apos;never in taxon&apos; value &apos;Aves&apos;</obo:IAO_0000112>
        <obo:IAO_0000115>x never in taxon T if and only if T is a class, and x does not instantiate the class expression &quot;in taxon some T&quot;. Note that this is a shortcut relation, and should be used as a hasValue restriction in OWL.</obo:IAO_0000115>
        <obo:IAO_0000117 rdf:resource="https://orcid.org/0000-0002-6601-2165"/>
        <obo:IAO_0000119 rdf:resource="http://www.ncbi.nlm.nih.gov/pubmed/17921072"/>
        <obo:IAO_0000119 rdf:resource="http://www.ncbi.nlm.nih.gov/pubmed/20973947"/>
        <obo:IAO_0000425>Class: ?X DisjointWith: RO_0002162 some ?Y </obo:IAO_0000425>
        <obo:OMO_0002000>PREFIX rdfs: &lt;http://www.w3.org/2000/01/rdf-schema#&gt;
PREFIX owl: &lt;http://www.w3.org/2002/07/owl#&gt;
PREFIX in_taxon: &lt;http://purl.obolibrary.org/obo/RO_0002162&gt;
PREFIX never_in_taxon: &lt;http://purl.obolibrary.org/obo/RO_0002161&gt;
CONSTRUCT {
  in_taxon: a owl:ObjectProperty .
  ?x owl:disjointWith [
    a owl:Restriction ;
    owl:onProperty in_taxon: ;
    owl:someValuesFrom ?taxon
  ] .
  ?x rdfs:subClassOf [
    a owl:Restriction ;
    owl:onProperty in_taxon: ;
    owl:someValuesFrom [
      a owl:Class ;
      owl:complementOf ?taxon
    ]
  ] .
}
WHERE {
  ?x never_in_taxon: ?taxon .
}</obo:OMO_0002000>
        <rdfs:isDefinedBy rdf:resource="http://purl.obolibrary.org/obo/phases/imports/ro_import.owl"/>
        <rdfs:label>never in taxon</rdfs:label>
        <rdfs:seeAlso rdf:resource="https://github.com/obophenotype/uberon/wiki/Taxon-constraints"/>
        <rdfs:subPropertyOf rdf:resource="http://purl.obolibrary.org/obo/RO_0002172"/>
    </owl:AnnotationProperty>
    


    <!-- http://purl.obolibrary.org/obo/RO_0002172 -->

    <owl:AnnotationProperty rdf:about="http://purl.obolibrary.org/obo/RO_0002172">
        <obo:IAO_0000115>An assertion that holds between an ontology class and an organism taxon class, which is intepreted to yield some relationship between instances of the ontology class and the taxon.</obo:IAO_0000115>
        <rdfs:isDefinedBy rdf:resource="http://purl.obolibrary.org/obo/phases/imports/ro_import.owl"/>
        <rdfs:label xml:lang="en">taxonomic class assertion</rdfs:label>
        <rdfs:seeAlso rdf:resource="https://github.com/obophenotype/uberon/wiki/Taxon-constraints"/>
        <rdfs:subPropertyOf rdf:resource="http://purl.obolibrary.org/obo/RO_0002420"/>
    </owl:AnnotationProperty>
    


    <!-- http://purl.obolibrary.org/obo/RO_0002416 -->

    <owl:AnnotationProperty rdf:about="http://purl.obolibrary.org/obo/RO_0002416">
        <obo:IAO_0000115>An assertion that involves at least one OWL object that is intended to be expanded into one or more logical axioms. The logical expansion can yield axioms expressed using any formal logical system, including, but not limited to OWL2-DL.</obo:IAO_0000115>
        <rdfs:isDefinedBy rdf:resource="http://purl.obolibrary.org/obo/phases/imports/ro_import.owl"/>
        <rdfs:label xml:lang="en">logical macro assertion</rdfs:label>
        <rdfs:seeAlso rdf:datatype="http://www.w3.org/2001/XMLSchema#anyURI">http://purl.obolibrary.org/obo/ro/docs/shortcut-relations/</rdfs:seeAlso>
    </owl:AnnotationProperty>
    


    <!-- http://purl.obolibrary.org/obo/RO_0002420 -->

    <owl:AnnotationProperty rdf:about="http://purl.obolibrary.org/obo/RO_0002420">
        <obo:IAO_0000115>A logical macro assertion whose domain is an IRI for a class</obo:IAO_0000115>
        <obo:IAO_0000116>The domain for this class can be considered to be owl:Class, but we cannot assert this in OWL2-DL</obo:IAO_0000116>
        <rdfs:isDefinedBy rdf:resource="http://purl.obolibrary.org/obo/phases/imports/ro_import.owl"/>
        <rdfs:label xml:lang="en">logical macro assertion on a class</rdfs:label>
        <rdfs:subPropertyOf rdf:resource="http://purl.obolibrary.org/obo/RO_0002416"/>
    </owl:AnnotationProperty>
    


    <!-- http://purl.org/dc/elements/1.1/contributor -->

    <owl:AnnotationProperty rdf:about="http://purl.org/dc/elements/1.1/contributor">
        <rdfs:isDefinedBy rdf:resource="http://purl.obolibrary.org/obo/phases/imports/ro_import.owl"/>
    </owl:AnnotationProperty>
    


    <!-- http://www.w3.org/2000/01/rdf-schema#comment -->

    <owl:AnnotationProperty rdf:about="http://www.w3.org/2000/01/rdf-schema#comment"/>
    


    <!-- http://www.w3.org/2000/01/rdf-schema#label -->

    <owl:AnnotationProperty rdf:about="http://www.w3.org/2000/01/rdf-schema#label"/>
    


    <!-- http://www.w3.org/2000/01/rdf-schema#seeAlso -->

    <owl:AnnotationProperty rdf:about="http://www.w3.org/2000/01/rdf-schema#seeAlso"/>
</rdf:RDF>



<!-- Generated by the OWL API (version 4.5.29) https://github.com/owlcs/owlapi -->

